%        File: a10_9.tex
%     Created: Di Dez 06 03:00  2016 C
% Last Change: Di Dez 06 03:00  2016 C
%
\documentclass[a4paper]{article}

\usepackage{amsmath, amssymb}

\title{Problem 10.9}
\author{Leul Shiferaw}

\begin{document}

\pagenumbering{gobble}
\maketitle
\newpage
\pagenumbering{arabic}

\begin{align*}
	&(\neg A\wedge \neg B \Rightarrow \neg(A\vee B))^f\\
	&(\neg A\wedge B)^t\\
	&\neg A^t\\
	&\neg B^t\\
	&A^f\\
	&(A\wedge B)^t\\
	&A^t\hspace{0.1cm}|\hspace{0.1cm} B^t\\
	&\perp \hspace{0.5cm}\perp
\end{align*}
Therefore the initial statement is not false(true)\\
\newpage
\begin{align*}
	&(A\Rightarrow B) \wedge (B\Rightarrow A\wedge B)^t\\
	&A\Rightarrow B^t\\
	&B\Rightarrow A\wedge B^t\\
\end{align*}
\begin{tabular}{|c|c|c|c|}
	&A$^f$&B$^t$&\\
	B$^f$ & A$\wedge$ B$^t$ & $B^f$ & A$\wedge$ B$^t$\\
	& A$^t$ & & A$^t$\\
	& && B$^t$\\
\end{tabular}
\\
$\indent\indent\hspace{0.2cm}\perp\hspace{1cm}\perp$
\\Continue to the table
\\\\$\therefore$ \{\{A$^f$, B$^f$\}, \{A$^t$, B$^t$\}\}
\end{document}
